correctness proof...almost

Logic/MultiSuccCorsiTassi/Kripke.lean
@@ -6,25 +6,76 @@ namespace multiSucc
 open multiSucc
 
 structure World where
-forced : List Atom
-unforced : List Atom
+  forced : Finset Atom
+  unforced : Finset Atom
+  -- prop : Disjoint forced unforced
+deriving DecidableEq
+--TODO PROOF OF MONOTONICITY. FORCED STAY FORCED. u is if c isnt in any.
+-- unforced vastupidi
+--wellFormed World
+def Seq4Proof.forced (s : Seq4Proof) : Finset Atom := s.as.toFinset
 
-def Seq4Proof.forced (s : Seq4Proof) : List Atom := s.as
+def Seq4Proof.unforced (s : Seq4Proof) : Finset Atom := s.bs.toFinset
 
-def Seq4Proof.unforced (s : Seq4Proof) : List Atom := s.bs
+def Seq4Proof.world (p : Seq4Proof) : World := ⟨p.forced, p.unforced \ p.forced⟩ -- , Finset.disjoint_sdiff⟩
 
-def Seq4Proof.world (p : Seq4Proof) : World := ⟨p.forced, p.unforced⟩
+-- attribute [grind .] World.prop
 
-structure CM where
-world : World
-branch : List CM
+
+structure Model where
+  world : World
+  branch : List Model
+deriving BEq
+
+--@[grind, simp]
+def Model.wf (m : Model) : Bool :=
+∀ fm ∈ m.branch.attach,
+  fm.val.wf ∧
+  m.world.forced ⊆ fm.val.world.forced ∧
+  fm.val.world.unforced ⊆ m.world.unforced
+decreasing_by
+all_goals
+  have : sizeOf m.branch < sizeOf m := by grind [Model]
+  apply lt_trans _ this
+  apply List.sizeOf_lt_of_mem
+  grind
+
+
+def Model.depth : Model → Nat
+| ⟨_, branch⟩ =>
+  1 + (branch.map Model.depth).max?.getD 0
+
+theorem Model.depth_eq {m : Model} : m.depth = 1 + (m.branch.map Model.depth).max?.getD 0 := by
+  cases m
+  simp [depth]
+
+lemma depth_lt_of_mem {m' m : Model} :
+  m' ∈ m.branch → m'.depth < m.depth := by
+  intro hmem
+  simp [Model.depth_eq]
+  have : m'.depth ∈ List.map Model.depth m.branch := by grind
+  have := List.le_max?_getD_of_mem this (k:=0)
+  simp [Model.depth_eq] at this
+  omega
+
+--@[grind, simp]
+def Model.all (m : Model) : List Model :=
+  m :: m.branch.attach.flatMap (all ·.val)
+decreasing_by
+  have : sizeOf m.branch < sizeOf m := by grind [Model]
+  apply lt_trans _ this
+  apply List.sizeOf_lt_of_mem
+  grind
+
+
+
 
 /--Truth Value: true, false, unknown -/
 inductive TV  where
 | t : TV
 | f : TV
 | u : TV
-deriving BEq
+deriving DecidableEq
 
 def conjTV : TV → TV → TV
 | .t, .t => .t
@@ -38,6 +89,30 @@ def disjTV : TV → TV → TV
 | _, .t => .t
 | _, _ => .u
 
+@[simp]
+theorem conjTV_left_false : conjTV .f a = b ↔ b = .f := by
+  grind [conjTV, cases TV]
+@[simp]
+theorem conjTV_right_false : conjTV a .f = b ↔ b = .f := by
+  grind [conjTV, cases TV]
+@[grind =, simp]
+theorem conjTV_true_iff : conjTV a b = .t ↔ a = .t ∧ b = .t := by
+  grind [conjTV, cases TV]
+@[grind =, simp]
+theorem conjTV_false_iff : conjTV a b = .f ↔ a = .f ∨ b = .f := by
+  grind [conjTV, cases TV]
+@[simp]
+theorem disjTV_left_false : disjTV .f a = b ↔ b = a := by
+  grind [disjTV, cases TV]
+@[simp]
+theorem disjTV_right_false : disjTV a .f = b ↔ b = a := by
+  grind [disjTV, cases TV]
+@[grind =, simp]
+theorem disjTV_true_iff : disjTV a b = .t ↔ a = .t ∨ b = .t := by
+  grind [disjTV, cases TV]
+@[grind =, simp]
+theorem disjTV_false_iff : disjTV a b = .f ↔ a = .f ∧ b = .f := by
+  grind [disjTV, cases TV]
 
 instance conjTV_rightCommutative : RightCommutative conjTV where
 right_comm a b c := by cases a <;> cases b <;> cases c <;> rfl
@@ -45,63 +120,492 @@ right_comm a b c := by cases a <;> cases b <;> cases c <;> rfl
 instance disjTV_rightCommutative : RightCommutative disjTV where
 right_comm a b c := by cases a <;> cases b <;> cases c <;> rfl
 
+instance conjTV_commutative : Std.Commutative conjTV where
+comm a b := by cases a <;> cases b <;> rfl
 
-/- def CM.depth : CM → Nat
-| ⟨_, branch⟩ => 1 + branch.length --root+children
- -/
-def CM.depth : CM → Nat
-| ⟨_, branch⟩ =>
-  1 + branch.foldl (fun m cm => max m cm.depth) 0
+instance disjTV_commutative : Std.Commutative disjTV where
+comm a b := by cases a <;> cases b <;> rfl
+
+instance conjTV_associative : Std.Associative conjTV where
+assoc a b c := by cases a <;> cases b <;> cases c <;> rfl
+
+instance disjTV_associative : Std.Associative disjTV where
+assoc a b c := by cases a <;> cases b <;> cases c <;> rfl
 
 
 
-lemma depth_lt_of_mem {cm' cm : CM} :
-  cm' ∈ cm.branch → cm'.depth < cm.depth := by
-  intro hmem
-  cases cm with
-  | mk w branch =>
-    simp [CM.depth]
-    sorry
 
-def evaluate : Form → CM → TV
-| .atoms a, cm => if a ∈ cm.world.forced then .t
-       else if a ∈ cm.world.unforced then .f
-       else dbg_trace "atom undefined"; .u
-| .bot, cm => .f
-| .and f g, cm => conjTV (evaluate f cm) (evaluate g cm )
-| .or f g, cm => disjTV (evaluate f cm) (evaluate g cm )
-| .imp f g, cm =>
-  if (evaluate f cm == .f || evaluate g cm == .t)
-      && (cm.branch.map (λ cm' => evaluate (f ⊃ g) cm' == .t)).all id then .t
-  else if (evaluate f cm == .t && evaluate g cm == .f)
-      || (cm.branch.map (λ cm' => evaluate (f ⊃ g) cm' == .f)).any id then .f --only one false
-  else dbg_trace "imp undefined";.u
-
-termination_by fm cm => (sizeOf_Form fm, cm.depth)
-decreasing_by
-all_goals first | (apply Prod.Lex.left; grind) | (apply Prod.Lex.right; apply depth_lt_of_mem; grind)
-
-def evalBlocked : Imp → CM → TV
-| {f, g}, cm =>
-  if (cm.branch.map (λ cm' => evaluate (f ⊃ g) cm' == .t)).all id then .t
-  else if (cm.branch.map (λ cm' => evaluate (f ⊃ g) cm' == .f)).any id then .f
+@[grind]
+def Form.eval : Form → Model → TV
+| .atoms a, m => if a ∈ m.world.forced then .t
+       else if a ∈ m.world.unforced then .f
+       else .u
+| .bot, _ => .f
+| .and a b, m => conjTV (a.eval m) (b.eval m )
+| .or a b, m => disjTV (a.eval m) (b.eval m )
+| .imp a b, m =>
+  if (a.eval m = .f ∨ b.eval m = .t)
+      ∧ (m.branch.all (λ m' => (a ⊃ b).eval m' = .t)) then .t
+  else if (a.eval m = .t ∧ b.eval m = .f)
+      ∨ (m.branch.any (λ m' => (a ⊃ b).eval m' = .f)) then .f --only one false
   else .u
+termination_by fm m => (sizeOf_Form fm, m.depth)
+decreasing_by
+all_goals first | (apply Prod.Lex.left; grind) | (apply Prod.Lex.right; apply depth_lt_of_mem; sorry)
 
-def evalAnt (Γ : List Form) (cm : CM) : TV :=
-match Γ with
-| []      => TV.t
-| f :: Γ' => conjTV (evaluate f cm) (evalAnt Γ' cm)
+@[grind, simp]
+def impTrueCond (a b : Form) (m : Model) : Prop :=
+  ((a.eval m = TV.f ∨ b.eval m = TV.t)) ∧
+  (m.branch.all (λ m' => (a ⊃ b).eval m' = TV.t))
 
-def evalSucc (Δ : List Form) (cm : CM) : TV :=
-match Δ with
-| []      => TV.f
-| f :: Δ' => disjTV (evaluate f cm) (evalSucc Δ' cm)
+@[grind, simp]
+def impFalseCond (a b : Form) (m : Model) : Prop :=
+  ((a.eval m = TV.t ∧ b.eval m = TV.f)) ∨
+  (m.branch.any (λ m' => (a ⊃ b).eval m' = TV.f))
 
+
+@[grind ., simp] theorem evalute_atom_t (h :  (Form.atoms a).eval m = .t) : a ∈ m.world.forced := by grind
+@[grind ., simp] theorem evalute_atom_f (h :  (Form.atoms a).eval m = .f) : a ∈ m.world.unforced := by grind
+@[grind ., simp] theorem evalute_atom_f_and (h :  (Form.atoms a).eval m = .f) : a ∈ m.world.unforced ∧ a ∉ m.world.forced:= by grind
+@[grind =, simp] theorem evalute_bot : Form.bot.eval m = .f := by grind
+@[grind =, simp] theorem evalute_and : (a ∧∧ b).eval m = conjTV (a.eval m) (b.eval m) := by grind
+@[grind =, simp] theorem evalute_or : (a ∨∨ b).eval m = disjTV (a.eval m) (b.eval m) := by grind
+@[grind =, simp]
+theorem evalute_atom_undef :
+    (Form.atoms a).eval m = .u ↔ a ∉ m.world.forced ∧ a ∉ m.world.unforced := by
+  grind
+
+
+/- def evalBlocked : Imp → Model → TV
+| {f, g}, m =>
+  if (m.branch.map (λ m' => (f ⊃ g).eval m' = .t)).all id then .t
+  else if (m.branch.map (λ m' => (f ⊃ g).eval m' = .f)).any id then .f
+  else .u -/
+
+
+def evalAnt (Γ : Multiset Form) (m : Model) : TV :=
+  (Γ.map (fun f => f.eval m)).fold conjTV TV.t
+
+scoped notation "⋀ " m:max ", " Γ:max => evalAnt Γ m
+
+def evalSucc (Δ : Multiset Form) (m : Model) : TV :=
+  (Δ.map (fun f => f.eval m)).fold disjTV TV.f
+
+scoped notation "⋁ " m:max ", " Γ:max => evalSucc Γ m
 
 -- A sequent is refutable iff all its assumptions are satisfied (all forms in Γ are true) but none of the conclusions are (all Δ are false)
-def evalSeq : Sequent /- → List Imp -/ → CM → TV
-| ⟨Γ, Δ ⟩, /- bl, -/ cm =>
-  match (evalAnt (Multiset.sort Γ LE.le) cm) , (evalSucc (Multiset.sort Δ LE.le) cm) with
-  | .u, _ | _, .u => .u
+@[grind]
+def evalSeq : Sequent /- → List Imp -/ → Model → TV
+| ⟨Γ, Δ ⟩, /- bl, -/ m =>
+  match (evalAnt Γ m) , (evalSucc Δ m) with
   | .t, .f => .f
-  | _, _ => .t
+  | .f, _ | _, .t => .t
+  | _, _ => .u
+
+
+lemma beq_f_true_eq {v : TV} :
+  (v = TV.f) → v = TV.f := by
+  cases v
+  . intro f; cases f
+  . grind
+  . intro f; cases f
+
+lemma beq_true_eq {x y : TV} :
+  (x = y) → x = y := by
+  intro h
+  cases x <;> cases y <;>  try cases h <;> rfl
+
+lemma beq_t_true_eq {v : TV} :
+  (v = TV.t) → v = TV.t := by
+  cases v
+  . grind
+  . intro f; cases f
+  . intro f; cases f
+
+@[simp]
+theorem evalSeq_true_iff :
+  evalSeq s m = TV.t ↔
+  evalAnt s.Γ m = TV.f ∨ evalSucc s.Δ m = TV.t := by
+  grind
+
+@[simp]
+theorem evalSeq_false_iff :
+  evalSeq s m = TV.f ↔
+  evalAnt s.Γ m = TV.t ∧ evalSucc s.Δ m = TV.f := by
+  simp [evalSeq]
+  split <;> grind
+
+@[grind ., simp]
+lemma evalAnt_not_t (h : x ∈ ys) (hx : x.eval m = .u) : ¬evalAnt ys m = TV.t := by
+  induction ys using Multiset.induction with
+  | empty => simp at h
+  | cons y ys ih =>
+    simp_all
+    rcases h with (⟨⟨_⟩⟩ | h)
+    · simp_all [evalAnt]
+    · simp_all [evalAnt]
+
+@[grind ., simp]
+lemma evalSucc_not_f (h : x ∈ ys) (hx : x.eval m = .u) : ¬⋁ m, ys = TV.f := by
+  induction ys using Multiset.induction with
+  | empty => simp at h
+  | cons y ys ih =>
+    simp_all
+    rcases h with (⟨⟨_⟩⟩ | h)
+    · simp_all [evalSucc]
+    · simp_all [evalSucc]
+
+@[grind =, simp]
+lemma evalSucc_bot_cons : ⋁ m, ↑(⊥ :: xs) = ⋁ m, ↑xs := by
+  simp [evalSucc]
+
+@[grind =, simp]
+lemma evalAnt_bot_cons : ⋀ m, ↑(⊥ :: xs) = .f := by
+  simp [evalAnt]
+
+@[grind =, simp]
+lemma evalAnt_conj : ⋀ m, ↑((a ∧∧ b) :: xs) = ⋀ m, ↑(a :: b :: xs) := by
+  simp [evalAnt]; grind
+
+@[grind =, simp]
+lemma evalSucc_conj : ⋁ m, ↑((a ∨∨ b) :: xs) = ⋁ m, ↑(a :: b :: xs) := by
+  simp [evalSucc]; grind
+
+@[grind =, simp]
+lemma evalSucc_cons {xs : List Form} :
+    ⋁ m, ↑(a :: xs) = disjTV (a.eval m) (⋁ m, ↑xs) := by
+  simp [evalSucc]
+
+@[grind =, simp]
+lemma evalAnt_cons {xs : List Form} :
+    ⋀ m, ↑(a :: xs) = conjTV (a.eval m) (⋀ m, ↑xs) := by
+  simp [evalAnt]
+
+@[grind =, simp]
+lemma evalAnt_eq_true :
+    ⋀ m, xs = .t ↔ ∀ x ∈ xs, x.eval m = .t := by
+  induction xs using Multiset.induction with simp_all [evalAnt]
+@[grind =, simp]
+lemma evalAnt_eq_false :
+    ⋀ m, xs = .f ↔ ∃ x ∈ xs, x.eval m = .f := by
+  induction xs using Multiset.induction with simp_all [evalAnt]
+
+@[grind =, simp]
+lemma evalSucc_eq_true :
+    ⋁ m, xs = .t ↔ ∃ x ∈ xs, x.eval m = .t := by
+  induction xs using Multiset.induction with simp_all [evalSucc]
+@[grind =, simp]
+lemma evalSucc_eq_false :
+    ⋁ m, xs = .f ↔ ∀ x ∈ xs, x.eval m = .f := by
+  induction xs using Multiset.induction with simp_all [evalSucc]
+
+@[grind ., simp]
+lemma evalSucc_true (fin : f ∈ Δ ) (ev : f.eval m = TV.t ): evalSucc Δ m = TV.t := by
+ simp; grind
+@[grind ., simp]
+lemma evalAnt_false (h₁ : f ∈ Γ) (h₂ : f.eval m = TV.f) : evalAnt Γ m = TV.f := by
+  simp; grind
+
+
+lemma eval_if_else_false {a b : Form} :
+  ((if ((a.eval m = TV.f) ∨ (b.eval m = TV.t)) ∧ ∀ x ∈ m.branch, ((a ⊃ b).eval x = TV.t) then TV.t
+  else if (a.eval m = TV.t) ∧ (b.eval m = TV.f) ∨ ∃ x ∈ m.branch, ((a ⊃ b).eval x = TV.f) then TV.f
+  else TV.u) =
+  TV.f) → (a.eval m = TV.t) ∧ (b.eval m = TV.f) ∨ ∃ x ∈ m.branch, ((a ⊃ b).eval x = TV.f) := by
+  intro h
+  split_ifs at h
+  . grind
+
+
+
+lemma eval_if_else_true {a b : Form}
+  (ifss : ((if ((a.eval m = TV.f) ∨ (b.eval m = TV.t)) ∧ ∀ x ∈ m.branch, ((a ⊃ b).eval x = TV.t) then TV.t
+  else if (a.eval m = TV.t) ∧ (b.eval m = TV.f) ∨ ∃ x ∈ m.branch, ((a ⊃ b).eval x = TV.f) then TV.f
+  else TV.u) =
+  TV.t)) : ((a.eval m = TV.f) ∨ (b.eval m = TV.t)) ∧ ∀ x ∈ m.branch, ((f ⊃ g).eval x = TV.t) := by
+
+
+  sorry
+
+
+--IMP EVAL--
+@[grind =, simp]
+theorem eval_imp_false_local :
+  a.eval m = .t → b.eval m = .f → (a ⊃ b).eval m = .f  := by
+  intro h₁ h₂; rw [Form.eval]; rw [h₁, h₂] ; simp
+
+@[grind =, simp]
+theorem eval_imp_true_if {a b : Form} : ((a.eval m = .f ∨ b.eval m = .t)
+      ∧ (m.branch.all (λ m' => (a ⊃ b).eval m' = .t))) → (a ⊃ b).eval m = .t := by grind [Form.eval]
+
+@[grind =, simp]
+theorem eval_imp_true_orl {a b : Form} {m : Model} :
+  (a.eval m = .f /- ∨ g.eval m = .t -/) → (m.branch.all (λ m' => (a ⊃ b).eval m' = .t)) → (a ⊃ b).eval m = .t := by
+  intro h₁ h₂
+  rw [Form.eval]; simp_all
+
+@[grind =, simp]
+theorem eval_imp_true_orr {a b : Form} :
+  (b.eval m = .t) → (m.branch.all (λ m' => (a ⊃ b).eval m' = .t)) → (a ⊃ b).eval m = .t := by
+  intro h₁ h₂
+  rw [Form.eval]; simp_all
+
+-- IN USE
+@[grind ., simp]
+theorem eval_imp_true_then (h₁ : (a ⊃ b).eval m = .t) :
+  (a.eval m = .f ∨ b.eval m = .t)
+      ∧ (m.branch.all (λ m' => (a ⊃ b).eval m' = .t)) := by grind [Form.eval]
+
+--@[grind ., simp]
+theorem eval_imp_false_if {a b : Form} :
+(a.eval m = .t ∧  b.eval m = .f ∨ ∃ x ∈ m.branch, ((a ⊃ b).eval x = TV.f)) →
+  (a ⊃ b).eval m = TV.f := by grind [Form.eval]
+
+--@[grind ., simp]
+theorem eval_imp_false_then :
+  (a ⊃ b).eval m = TV.f → a.eval m = .t ∧  b.eval m = .f ∨ ∃ x ∈ m.branch, ((a ⊃ b).eval x = TV.f) := by
+    intro h;
+    rw [Form.eval] at h
+    simp_all
+    apply eval_if_else_false at h
+    exact h
+
+-- IN USE
+theorem eval_imp_righ_wo_ys :
+  evalSeq { Γ := ↑xs, Δ := {a ⊃ b} } m ≠ TV.f →
+  evalSeq { Γ := ↑xs, Δ := ↑((a ⊃ b) :: ys) } m ≠ TV.f := by
+  simp; intro h₁ h₂; simp_all
+
+-- IN USE
+-- TODO CHANGE TO IFF?? TODO changed to .branch not .all. Thoughts?
+@[grind ., simp]
+theorem eval_imp_false_contradict :
+  (a ⊃ b).eval m = TV.f → ∃ m' ∈ m.all, a.eval m' = .t ∧ b.eval m' = .f := by
+  intro impF
+  fun_induction Model.all with
+  | case1 m ih =>
+    apply eval_imp_false_then at impF
+    rcases impF with impF | ⟨m', impF⟩
+    . grind
+    . simp_all
+      specialize ih m' (by grind) impF.right
+      obtain ⟨m'', ih⟩ := ih
+      grind
+
+/- @[grind ., simp]
+theorem eval_imp_false_iff :
+  (a ⊃ b).eval m = TV.f ↔ ∃ m' ∈ m.branch, a.eval m' = .t ∧ b.eval m' = .f := by
+  constructor
+  . intro h
+    apply eval_imp_false_then at h
+    rcases h with impF | ⟨m', impF⟩
+
+  . intro h
+    rcases h with ⟨m', h₁, h₂, h₃⟩
+    apply eval_imp_false_if
+    right
+    grind -/
+
+
+--MONOTONICITY--
+
+/-
+same as mode_branch_mono
+theorem mono_true_form {a : Form} {m : Model} :
+  ( a.eval m = .t) → (∀ x ∈ m.branch, a.eval x = .t)  := by sorry -/
+
+@[grind ., simp]
+theorem branch_mem_of_all {m m' a : Model} (h₁ : a ∈ m.branch) (h₂ : m' ∈ a.all) : m' ∈ m.all := by
+  fun_induction Model.all m with
+  | case1 m ih =>
+    simp_all
+    right
+    grind
+
+-- IN USE
+@[grind ., simp]
+theorem wf_of_mem_all {m m' : Model} (wf : m.wf) (mem : m' ∈ m.all) : m'.wf := by
+  fun_induction Model.all with
+  | case1 m ih =>
+    simp_all
+    rcases mem with h | ⟨a, h₁, h₂⟩
+    . grind
+    . rw [Model.wf] at wf
+      simp_all
+      apply ih a h₁ h₂
+
+--TODO IMPORTANT
+@[grind ., simp]
+theorem model_branch_mono_t {f : Form} {m m' : Model}
+  (wf : m.wf) (mem : m' ∈ m.branch) (ftv : f.eval m = TV.t) :
+    f.eval m' = TV.t := by
+  have h : ∀ a ∈ m.branch, a.wf = true ∧
+        m.world.forced ⊆ a.world.forced ∧
+        a.world.unforced ⊆ m.world.unforced := by
+      unfold Model.wf at wf; simp at wf; exact wf
+  specialize h m' mem
+  obtain ⟨mf', fo, unfo⟩ := h
+  match f with
+  | .atoms a => grind
+  | .bot => grind
+  | .and a b =>
+    simp_all
+    constructor
+    . obtain ⟨atv, btv⟩ := ftv
+      apply model_branch_mono_t wf mem
+      exact atv
+    . obtain ⟨atv, btv⟩ := ftv
+      apply model_branch_mono_t wf mem
+      exact btv
+  | .or a b =>
+    simp_all
+    cases ftv with
+    | inl h =>
+      left
+      apply model_branch_mono_t wf mem
+      exact h
+    | inr h =>
+      right
+      apply model_branch_mono_t wf mem
+      exact h
+  | .imp a b =>
+    apply eval_imp_true_then at ftv
+    obtain ⟨h₁, h₂⟩ := ftv
+    grind
+
+-- IN USE
+theorem model_all_mono {f : Form} {m m' : Model}
+  (wf : m.wf) (mem : m' ∈ m.all) (ftv : f.eval m = TV.t) :
+  f.eval m' = TV.t := by
+  rw [Model.all] at mem
+  --rw [Model.wf] at wf
+  simp_all
+  rcases mem with h | ⟨a, h₁, h₂⟩
+  . grind
+  . have wf' : m'.wf = true := wf_of_mem_all wf (by grind)
+    have aT := model_branch_mono_t wf h₁ ftv
+    have awf : a.wf := by
+      rw [Model.wf] at wf; simp at wf
+      grind
+    apply model_all_mono awf h₂ aT
+termination_by (m.depth)
+decreasing_by exact depth_lt_of_mem h₁
+
+-- IN USE
+@[grind ., simp]
+theorem model_all_mono_list {xs : List Form} {m m' : Model}
+  (wf : m.wf) (mem : m' ∈ m.all) (xstv : ∀ x ∈ xs, x.eval m = TV.t) :
+  ∀ x ∈ xs, x.eval m' = TV.t := by grind [model_all_mono]
+
+@[grind ., simp]
+theorem mono_false_form_branch {f : Form} {m m' : Model}
+  (wf : m.wf) (mem : m' ∈ m.branch ) (ftv : f.eval m' = .f) :
+  f.eval m = .f  := by
+  have h : ∀ a ∈ m.branch, a.wf = true ∧
+        m.world.forced ⊆ a.world.forced ∧
+        a.world.unforced ⊆ m.world.unforced := by
+      unfold Model.wf at wf; simp at wf; exact wf
+  specialize h m' mem
+  obtain ⟨mf', fo, unfo⟩ := h
+  match f with
+  | .atoms a =>
+    apply evalute_atom_f_and at ftv; simp [Form.eval]; grind -- NEED DISJONINT PROOF ?!!? NO???
+  | .bot => grind
+  | .and a b =>
+    simp_all
+    cases ftv with
+    | inl h =>
+      left
+      apply mono_false_form_branch wf mem
+      exact h
+    | inr h =>
+      right
+      apply mono_false_form_branch wf mem
+      exact h
+  | .or a b =>
+    simp_all
+    constructor
+    . obtain ⟨atv, btv⟩ := ftv
+      apply mono_false_form_branch wf mem
+      exact atv
+    . obtain ⟨atv, btv⟩ := ftv
+      apply mono_false_form_branch wf mem
+      exact btv
+  | .imp a b =>
+    apply eval_imp_false_if
+    right
+    use m'
+
+/- theorem mono_false_all_branch {f : Form} {m m' a : Model}
+  (wf : m.wf) (mem : a ∈ m.branch) (mem' : m' ∈ a.all ) (ftv : f.eval m' = .f)  :
+  f.eval a = .f := by
+  rw [Model.all] at mem'; simp at mem'
+  rcases mem' with id | ⟨mm, h₁, h₂⟩
+  . grind
+  . have awf : a.wf = true := by rw [Model.wf] at wf; simp at wf; grind
+    have mmwf : mm.wf = true := by rw [Model.wf] at awf; simp at awf; grind
+    sorry
+    --have : f.eval mm = .f := mono_false_form_branch mmwf mem ftv
+    --exact mono_false_all_branch (by sorry) h₁ h₂
+
+
+theorem mono_false_form_all {f : Form} {m m' : Model}
+  (wf : m.wf) (mem : m' ∈ m.all ) (ftv : f.eval m' = .f) :
+  f.eval m = .f  := by
+  rw [Model.all] at mem
+  simp_all
+  rcases mem with h | ⟨a, h₁, h₂⟩
+  . grind
+  . have h := mono_false_all_branch wf h₁ h₂ ftv
+    have wf' : m'.wf = true := wf_of_mem_all wf (by grind)
+    exact mono_false_form_branch wf h₁ h -/
+
+
+theorem imo_branch_false_then_b_false {a b : Form} {m m' : Model}
+(mem : m' ∈ m.branch) (h : (a ⊃ b).eval m' = TV.f) (wf : m.wf) :
+b.eval m = TV.f := by
+  apply eval_imp_false_then at h
+  rcases h with ⟨atv, btv⟩ | h
+  . exact mono_false_form_branch wf mem btv
+  . obtain ⟨x, xmem, h⟩ := h
+    have mwf : m'.wf = true := by rw [Model.wf] at wf; simp at wf; grind
+    have := imo_branch_false_then_b_false xmem h mwf
+    exact mono_false_form_branch wf mem this
+termination_by (m.depth)
+decreasing_by exact depth_lt_of_mem mem
+
+-- IN USE
+theorem eval_imp_false_then_b_false  (impF : (a ⊃ b).eval m = TV.f) (wf : m.wf) : b.eval m = .f := by
+  apply eval_imp_false_then at impF
+  cases impF with
+  | inl h => grind
+  | inr h =>
+    rcases h with ⟨m', mem, h₂⟩
+    exact imo_branch_false_then_b_false mem h₂ wf
+
+
+
+/- theorem Model_monotonicity_t {m: Model} : ∀ fm ∈ m.branch, m.world.forced ⊆ fm.world.forced := by sorry
+theorem Model_monotonicity_f {m: Model} : ∀ fm ∈ m.branch, fm.world.unforced ⊆ m.world.unforced := by sorry
+ -/
+/-
+@[simp]
+theorem eval_imp_false_future {m : Model} {h : m.wf} {a b : Form}:
+  (∃ x ∈ m.branch, ((a ⊃ b).eval x = TV.f)) →
+  (a ⊃ b).eval m = .f := by
+  sorry -/
+
+/- @[grind ., simp]
+theorem eval_imp_not_false_then :
+  (¬(a ⊃ b).eval m = TV.f) →
+  impTrueCond a b m ∨ (¬ impTrueCond a b m ∧ ¬ impFalseCond a b m) := by
+  intro h; rw [Form.eval] at h; simp at h
+  by_cases hT :
+  ((a.eval m = TV.f) ∨ (b.eval m = TV.t)) ∧
+  ∀ x ∈ m.branch, ((a ⊃ b).eval x = TV.t)
+  · left
+    exact hT
+  · right
+    constructor
+    · intro hT'; grind
+    · sorry -/
