Logic/MultiSuccDyckhoff/Core.lean
@@ -1,4 +1,6 @@
 import Mathlib.Data.Multiset.Basic
+import Mathlib.Data.Multiset.Sort
+import Mathlib.Data.List.Lex
 
 namespace multiSucc
 
@@ -14,6 +16,15 @@ inductive Form
 | imp : Form → Form → Form
 deriving DecidableEq, Repr
 
+structure Imp where
+  left : Form
+  right : Form
+deriving DecidableEq, Repr
+
+structure aImp where
+  a : Atom
+  f : Form
+
 -- such notation is used as not to confuse with Lean's internal logic notation
 notation "⊥" => Form.bot
 infixl:50 " ∧∧ " => Form.and
@@ -22,22 +33,97 @@ infixl:60 " ⊃ " => Form.imp
 
 def Form.neg (a : Form) : Form :=  a ⊃ ⊥
 
-inductive Sequent
-  | seq : Multiset Form → Multiset Form → Sequent
+@[simp, grind]
+def Imp.toForm (i : Imp) : Form :=
+  i.left ⊃ i.right
 
---TODO irreducable sequent
+def aImp.toForm (i : aImp) : Form :=
+  .atoms i.a ⊃ i.f
+
+structure Sequent where
+  Γ : Multiset Form
+  Δ : Multiset Form
+
+
 /-
 Seq4Proof is needed to seperate the purely atomic formulas from the rest in antecedent.
 This is required for easier algorithmic approach, where we can one by one open up the more complex formulas.
 Seperate atomic implications in the form a → P, bc these need to be handled last.
 atoms, forms, imps, aimps ⊢ atoms, forms, imps
-[x, y], [f1, f2], [imp1, imp2] [aImp] ⊢ [x, y], [g1, g2], [imp1, imp2]
+[x, y], [f1, f2] [aImp] ⊢ [x, y], [g1, g2], [imp1, imp2]
  -/
+structure Seq4proof where
+  as : List Atom
+  fL : List Form
+  aimp : List aImp
+  bs : List Atom
+  fR : List Form
+  impR : List Imp
 
- -- TODO maybe make seperate type Imp and specify which lists are Imp Lists
-inductive Seq4Proof
-  | seq4 : List Atom → List Form → List Form → List Form → List Atom → List Form → List Form → Seq4Proof
---deriving Repr
+/- def Seq4Proof.irreducable : Seq4Proof → Bool
+| {as, [], aimp, bs, [], impR} =>
+  if no a ∈ as in left of ∀  imp ∈  aimps -/
+
+@[simp]
+def Form.encode : Form → List Nat
+  | bot        => [0]
+  | atoms a    => [1, a.atom]
+  | and f g    => [2, (encode f).length] ++ encode f ++ encode g
+  | or f g     => [3, (encode f).length] ++ encode f ++ encode g
+  | imp f g    => [4, (encode f).length] ++ encode f ++ encode g
+
+lemma Atom.ext {a b : Atom} (h : a.atom = b.atom) : a = b := by
+  cases a; cases b
+  simp_all
+
+theorem form_inj {f : Form} (h : f.encode = g.encode) :
+  f = g := by
+  match f, g with
+  | .bot, .bot => rfl
+  | .bot, .atoms _ => simp only [Form.encode, List.cons.injEq, Nat.zero_ne_one, List.ne_cons_self,
+    and_self] at h
+  | .atoms _, .bot => simp only [Form.encode, List.cons.injEq, Nat.succ_ne_self, List.cons_ne_self,
+    and_self] at h
+  | .atoms a, .atoms b =>
+    simp only [Form.encode, List.cons.injEq, and_true, true_and] at h
+    apply congrArg Form.atoms (Atom.ext h)
+  | .and f g, .and f' g' =>
+    simp_all only [Form.encode, List.cons_append, List.nil_append, List.cons.injEq, true_and,
+      Form.and.injEq]
+    let ⟨h1,h2⟩ := h
+    have := List.append_inj_right h2 h1
+    have hn := List.append_inj_left' h2 (congrArg List.length this)
+    exact ⟨form_inj hn, form_inj this⟩
+  | .or f g, .or f' g' =>
+    simp_all only [Form.encode, List.cons_append, List.nil_append, List.cons.injEq, true_and,
+      Form.or.injEq]
+    let ⟨h1,h2⟩ := h
+    have := List.append_inj_right h2 h1
+    have hn := List.append_inj_left' h2 (congrArg List.length this)
+    exact ⟨form_inj hn, form_inj this⟩
+  | .imp f g, .imp f' g' =>
+    simp_all only [Form.encode, List.cons_append, List.nil_append, List.cons.injEq, true_and,
+      Form.imp.injEq]
+    let ⟨h1,h2⟩ := h
+    have := List.append_inj_right h2 h1
+    have hn := List.append_inj_left' h2 (congrArg List.length this)
+    exact ⟨form_inj hn, form_inj this⟩
+
+instance : LinearOrder Atom :=
+  LinearOrder.lift' (fun a : Atom => a.atom) (fun _ _ h => Atom.ext h)
+
+instance : LinearOrder Form :=
+  LinearOrder.lift' Form.encode (fun _ _ h => form_inj h)
+
+
+@[simp]
+def Seq4Proof.toSeq (p : Seq4proof ) : Sequent :=
+  have ant := Multiset.ofList ((p.as.map .atoms) ++ p.fL ++ p.aimp.map aImp.toForm)
+  have succ := Multiset.ofList ((p.bs.map .atoms) ++ p.fR ++ p.impR.map Imp.toForm)
+  ⟨ant, succ⟩
+
+def Sequent.toSeq4 (s : Sequent) : Seq4proof :=
+Seq4proof.mk [] (Multiset.sort s.Γ LE.le) [] [] (Multiset.sort s.Δ LE.le) []
 
 
 end multiSucc
