Logic/MultiSuccCorsiTassi/Correctness.lean
@@ -1,21 +1,86 @@
 import Logic.MultiSuccCorsiTassi.Core
-import Logic.MultiSuccCorsiTassi.Syntax
+--import Logic.MultiSuccCorsiTassi.Syntax
 import Logic.MultiSuccCorsiTassi.Helper
-import Logic.MultiSuccCorsiTassi.Display
+--import Logic.MultiSuccCorsiTassi.Display
 import Logic.MultiSuccCorsiTassi.Kripke
-import Logic.MultiSuccCorsiTassi.MultiSuccCorsiTassi
+--import Logic.MultiSuccCorsiTassi.MultiSuccCorsiTassi
+import Logic.MultiSuccCorsiTassi.Proof
 
 namespace multiSucc
 open multiSucc
 
-theorem CM_ertyu : ∀ cm : CM, cm.world.forced ∩ cm.world.unforced = ∅ := by sorry
-theorem CM_true_in_future : ∀ (cm : CM), cm.world.forced ∈ cm.branch.map (λ child ↦ child.world.forced) := by sorry
+theorem Model_ertyu : ∀ m : Model, m.world.forced ∩ m.world.unforced = ∅ := by sorry
+theorem Model_true_in_future : ∀ (m : Model), m.world.forced ∈ m.branch.map (λ child ↦ child.world.forced) := by sorry
 
 
 /-- If a sequent gets  countermodels as results, each of those models must refute the sequent  -/
-theorem CM_correctness :
-  ∀ (s : Sequent) {capProof} {metaR1} (cms : List CM),
-    automatedProof s.toSeq4 s.toSeq4.cap.card capProof metaR1 = Result.cm cms →
-    ∀ cm ∈ cms, evalSeq s cm = TV.f := by
-    intro s proof r1 cms res c h
-    simp [evalSeq, conjTV, disjTV, evaluate]; sorry
+/- theorem Model_correctness :
+  ∀ (s : Sequent) {capProof} {metaR1} (ms : List Model),
+    automatedProof s.toSeq4 s.toSeq4.cap.card capProof metaR1 = Result.m ms →
+    ∀ m ∈ ms, evalSeq s m = TV.f := by
+    intro s proof r1 ms res c h
+    simp [evalSeq, conjTV, disjTV, Form.eval]; sorry -/
+
+
+
+--TODO if all atoms in stuctures every world, then eval = .t
+-- if eval u, then some atom ....
+-- sequent holds if for all structures
+theorem proof_correctness :
+  ∀ (s : Sequent) (_ : Proof s) (m : Model) (_ : m.wf), evalSeq s m ≠ TV.f := by
+  intro s pf m wf
+  induction pf generalizing m with
+  | ax x xs ys hxs hys =>
+    simp only [ne_eq, evalSeq_false_iff, Classical.not_and_iff_not_or_not]
+    have hxsM : Form.atoms x ∈ (↑xs : Multiset Form) := by simpa using hxs
+    if xtv : x ∈ m.world.forced then
+      suffices evalSucc ↑ys m = TV.t by grind
+      apply evalSucc_true hys
+      grind
+    else if xtv' : x ∈ m.world.unforced then grind
+    else grind
+  | botl => grind
+  | botr xs ys prem => simp_all
+  | andl a b xs ys prem ih =>
+    simp_all
+  | andr a b xs ys prem1 prem2 =>
+    simp_all only [ne_eq, evalSeq_false_iff]
+    grind
+  | orl a b xs ys prem1 prem2 =>
+    simp_all only [ne_eq, evalSeq_false_iff, evalAnt_cons, not_and]
+    grind
+  | orr a b xs ys prem =>
+    simp_all
+  | impr a b xs ys prem ih => --tahame et a b oleks t,a on f u, b t, u
+    apply eval_imp_righ_wo_ys
+    simp_all--ih gives that b cant be false. ys throw away. ih on ms children as well to show that future imp is false
+    intro h₁ impF
+    apply eval_imp_false_contradict at impF
+    --simp_all
+    contrapose! ih
+    simp_all
+    rcases impF with ⟨m', hm_mem, ⟨ha, hb⟩⟩
+    . use m'
+      have aaaa := model_all_mono_list wf hm_mem h₁
+      simp_all
+      apply wf_of_mem_all wf hm_mem
+
+  | impl a b xs ys prem1 prem2 ih₁ ih₂ =>
+    simp_all
+    intro h₁ h₂
+    have impT := eval_imp_true_then h₁
+    simp at impT
+    cases impT with
+    | intro himp hbranch =>
+      cases himp with
+      | inl h => exact Set.inter_nonempty.mp (ih₁ m wf h₁ h₂ h)
+      | inr h => simp_all
+
+  | afort a b xs ys prem ih =>
+    simp_all
+    intro h₁ h₂
+    specialize ih m wf h₁
+    apply_assumption
+    apply eval_imp_false_then_b_false h₂
+
+#print axioms proof_correctness
