Logic/MultiSuccCorsiTassi/Proof.lean
@@ -1,0 +1,120 @@
+
+import Logic.MultiSuccCorsiTassi.Core
+import Logic.MultiSuccCorsiTassi.Helper
+import Logic.MultiSuccCorsiTassi.Display
+
+namespace multiSucc
+open multiSucc
+/-
+Multi-succedent formulas.
+Added a fortiori
+ -/
+inductive Proof : Sequent → Type
+  -- ∀ x Γ, x ++ Γ ⊢ x ++ Δ
+  | ax :
+    ∀ (x : Atom) (xs ys: List Form),
+      (hxs : .atoms x ∈ xs) →
+      (hys : .atoms x ∈ ys) →
+      Proof ⟨↑xs, ↑ys⟩
+  -- ∀ Δ Γ, (⊥, Γ ⊢ Δ)
+  | botl :
+    ∀ (xs ys : List Form),
+      Proof ⟨↑(⊥ :: xs), ↑ys⟩
+  | botr :
+    ∀ (xs ys : List Form),
+      Proof ⟨↑xs, ↑ys⟩ →
+      Proof ⟨↑xs, ↑(⊥ :: ys)⟩
+  -- ∀ a b Γ Δ, (Γ, a, b ⊢ Δ) → (Γ, a ∧ b ⊢ Δ)
+  | andl :
+    ∀ (a b : Form) (xs ys: List Form),
+      Proof ⟨↑(a :: b :: xs), ↑ys⟩ →
+      Proof ⟨↑((a ∧∧ b) :: xs), ↑ys⟩
+  -- ∀ a b Γ Δ, (Γ ⊢ a, Δ) → (Γ ⊢ b, Δ) → (Γ ⊢ a ∧ b, Δ)
+  | andr :
+    ∀ (a b : Form) (xs ys: List Form),
+      Proof ⟨↑xs, ↑(a :: ys)⟩ →
+      Proof ⟨↑xs, ↑(b :: ys)⟩ →
+      Proof ⟨↑xs, ↑((a ∧∧ b) :: ys)⟩
+  -- ∀ a b Γ Δ, (a, Γ ⊢ Δ) → (b, Γ ⊢ Δ) → (a ∨ b, Γ ⊢ Δ)
+  | orl :
+    ∀ (a b : Form) (xs ys : List Form),
+    Proof ⟨↑(a :: xs), ↑ys⟩ →
+    Proof ⟨↑(b :: xs), ↑ys⟩ →
+    Proof ⟨↑((a ∨∨ b) :: xs), ↑ys⟩
+  -- ∀ a b Γ Δ , (Γ ⊢ a, b, Δ) → (Γ ⊢ a ∨ b, Δ)
+  | orr :
+    ∀ (a b : Form) (xs ys : List Form),
+      Proof ⟨↑xs, ↑(a :: b :: ys)⟩ →
+      Proof ⟨↑xs, ↑(( a ∨∨ b) :: ys)⟩
+  -- ∀ a b Γ Δ, (a, Γ ⊢ b) → ( Γ ⊢ a → b, Δ)
+  | impr :
+    ∀ (a b : Form) (xs ys: List Form),
+      Proof ⟨↑(a :: xs), {b}⟩ →
+      Proof ⟨↑(xs), ↑((a ⊃ b) :: ys)⟩
+  -- ∀ a b Γ Δ, (a → b, Γ ⊢ a, Δ) → (b, Γ ⊢ Δ) → (a → b, Γ ⊢ Δ)
+  | impl :
+    ∀ (a b : Form) (xs ys : List Form),
+      Proof ⟨↑((a ⊃ b) :: xs), ↑(a :: ys)⟩ →
+      Proof ⟨↑(b :: xs ), ↑ys⟩ →
+      Proof ⟨↑((a ⊃ b) :: xs), ↑ys⟩
+  -- ∀ a b Γ Δ, (Γ ⊢ b, Δ) → (Γ ⊢ a → b, Δ)
+  | afort :
+    ∀ (a b : Form) (xs ys : List Form),
+      Proof ⟨↑xs, ↑(b :: ys)⟩ →
+      Proof ⟨↑xs, ↑((a ⊃ b) :: ys)⟩
+
+
+
+
+def proofToString  {xseq : Sequent} (indentLvl : Nat) : Proof xseq → String
+| .ax _ xs ys _ _=>
+  indent indentLvl s!"AX: {listToString xs} ⊢ {listToString ys}"
+| .botl xs ys =>
+  indent indentLvl s!"⊥L: ⊥, {listToString xs} ⊢ {listToString ys}"
+| .botr xs ys proof =>
+  let premise := proofToString (indentLvl + 1) proof
+  let ruleLine :=
+  s!"⊥R: {listToString xs} ⊢ ⊥, {listToString ys}"
+  s!"{premise}\n{indent indentLvl (horizontalLine ruleLine.length)}\n{indent indentLvl ruleLine}"
+| .andl a b xs ys proof =>
+  let premise := proofToString (indentLvl + 1) proof
+  let ruleLine := s!"∧L: ({a} ∧ {b}), {listToString xs} ⊢ {listToString ys}"
+  s!"{premise}\n{indent indentLvl (horizontalLine ruleLine.length)}\n{indent indentLvl ruleLine}"
+| .andr a b xs ys proof₁ proof₂=>
+  let left := proofToString  (indentLvl + 1) proof₁
+  let right := proofToString (indentLvl + 1) proof₂
+  let ruleLine := s!"∧R: {listToString xs} ⊢ {a} ∧ {b}, {listToString ys}"
+  s!"{left}\n{right}\n{indent indentLvl (horizontalLine (ruleLine.length))}\n{indent indentLvl ruleLine}"
+| .orl a b xs ys proof₁ proof₂=>
+  let left := proofToString  (indentLvl + 1) proof₁
+  let right := proofToString (indentLvl + 1) proof₂
+  let ruleLine := s!"∨L: ({a} ∨ {b}), {listToString xs} ⊢ {listToString ys}"
+  s!"{left}\n{right}\n{horizontalLine (ruleLine.length)}\n{indent indentLvl ruleLine}"
+| .orr a b xs ys proof =>
+  let premise := proofToString (indentLvl + 1) proof
+  let ruleLine := s!" ∨R: {listToString xs} ⊢ {a} ∨ {b}, {listToString ys}"
+  s!"{ premise}\n{indent indentLvl (horizontalLine ruleLine.length)}\n{indent indentLvl ruleLine}"
+| .impl a b xs ys proof₁ proof₂ =>
+  let left  := proofToString (indentLvl + 1) proof₁
+  let right := proofToString (indentLvl + 1) proof₂
+  let ruleLine := s!"→L: ({a} → {b}), {listToString xs}⊢ {listToString ys}"
+  s!"{left}\n{right}\n{indent indentLvl (horizontalLine ruleLine.length)}\n{indent indentLvl ruleLine}"
+| .impr a b xs ys proof  =>
+  let premise := proofToString (indentLvl + 1) proof
+  let ruleLine := s!"→R: {listToString xs} ⊢ {a} → {b}, {listToString ys}"
+  s!"{ premise}\n{indent indentLvl (horizontalLine ruleLine.length)}\n{indent indentLvl ruleLine}"
+| .afort a b xs ys proof  =>
+  let premise := proofToString (indentLvl + 1) proof
+  let ruleLine := s!"→AF: {listToString xs} ⊢ {a} → {b}, {listToString ys}"
+  s!"{premise}\n{indent indentLvl (horizontalLine ruleLine.length)}\n{indent indentLvl ruleLine}"
+
+
+
+
+def listProofToString : List (Proof xseq) → String
+| [] => ""
+| x::xs => (proofToString 0 x).replace " ," "" ++ "\n \n" ++ listProofToString xs
+
+
+instance : ToString (List (Proof xseq)) where
+  toString proof := listProofToString proof
